WebAssembly/Wasm_Monad_Assertions.thy
@@ -122,4 +122,29 @@ definition cfg_m_assn :: "inst_store \<Rightarrow> config \<Rightarrow> config_m
    * inst_store_assn i_s
 )"     
 
+
+
+(* misc triples *)
+
+abbreviation "fits_at_in l n la \<equiv> case l of [] \<Rightarrow> True | x#xs \<Rightarrow> n+length l \<le> length la"
+
+abbreviation "insert_at_in l n la \<equiv> take n la @ l @ drop (n+length l) la"
+
+lemma list_blit_array_triple:
+  "<a \<mapsto>\<^sub>a la> 
+  list_blit_array l a n
+  <\<lambda>r. \<up>(fits_at_in l n la) 
+    * a \<mapsto>\<^sub>a insert_at_in l n la>"
+proof(induct l arbitrary:a la n)
+case Nil
+  then show ?case by sep_auto
+next
+  case (Cons a l)
+  show ?case 
+    supply [simp del] = list_blit_array.simps
+    apply(subst list_blit_array.simps)
+    apply(sep_auto heap:Cons split:list.splits simp: take_update_last)
+    done
+qed
+
 end
